Phi_System/Phi_Types.thy
@@ -2062,9 +2062,9 @@ subsubsection \<open>Reasoning\<close>
 lemma \<phi>Mul_Quant\<^sub>\<Lambda>_wrap_module_src:
   \<open> \<g>\<u>\<a>\<r>\<d> (\<c>\<o>\<n>\<d>\<i>\<t>\<i>\<o>\<n> y' i = fst y \<and> i \<in> I \<longrightarrow> ((fst x, w) \<Ztypecolon> T \<^emph>[C\<^sub>W] W \<t>\<r>\<a>\<n>\<s>\<f>\<o>\<r>\<m>\<s> y \<Ztypecolon> U i \<^emph>[C\<^sub>R] R i \<w>\<i>\<t>\<h> P))
        \<and>\<^sub>\<r> \<c>\<o>\<n>\<d>\<i>\<t>\<i>\<o>\<n> i \<in> I
-\<Longrightarrow> \<p>\<r>\<e>\<m>\<i>\<s>\<e> y' i = fst y
-\<Longrightarrow> ((snd x) \<Ztypecolon> \<half_blkcirc>[C\<^sub>W'] W) = ((w, y') \<Ztypecolon> \<half_blkcirc>[C\<^sub>W] W \<^emph> \<half_blkcirc>[True] (\<big_ast>\<^sup>\<phi> (I - {i}) U)) @action \<A>merge
-\<Longrightarrow> x \<Ztypecolon> T \<^emph>[C\<^sub>W'] W \<t>\<r>\<a>\<n>\<s>\<f>\<o>\<r>\<m>\<s> (y', snd y) \<Ztypecolon> \<big_ast>\<^sup>\<phi> I U \<^emph>[C\<^sub>R] R i \<w>\<i>\<t>\<h> P \<close>
+\<Longrightarrow> \<p>\<r>\<e>\<m>\<i>\<s>\<e> y' i = fst y \<and> (\<forall>i \<in> I - {i}. y'' i = y' i)
+\<Longrightarrow> ((snd x) \<Ztypecolon> \<half_blkcirc>[C\<^sub>W'] W') = ((w, y'') \<Ztypecolon> \<half_blkcirc>[C\<^sub>W] W \<^emph> \<half_blkcirc>[True] (\<big_ast>\<^sup>\<phi> (I - {i}) U)) @action \<A>merge
+\<Longrightarrow> x \<Ztypecolon> T \<^emph>[C\<^sub>W'] W' \<t>\<r>\<a>\<n>\<s>\<f>\<o>\<r>\<m>\<s> (y', snd y) \<Ztypecolon> \<big_ast>\<^sup>\<phi> I U \<^emph>[C\<^sub>R] R i \<w>\<i>\<t>\<h> P \<close>
   unfolding Action_Tag_def \<r>Guard_def Ant_Seq_imp
   apply (simp add: cond_prod_transformation_rewr,
          simp add: \<phi>Prod_expn'' \<phi>Prod_expn' \<phi>Some_\<phi>Prod[symmetric] Cond_\<phi>Prod_expn_\<phi>Some)
